transfer

examples/BinarySearchTree.v
@@ -66,7 +66,6 @@ Module BinaryTreeModel(A : BINARY_TREE_ASSOCIATION).
       match goal with
         | [H1: ?e, H2: ?e |- _] => clear H2 || clear H1
         | [H1: ?a = ?b, H2:?b = ?a |- _] => clear H2 || clear H1
-        | [H: Some _ = Some _ |- _] => inversion H; clear H
         | [ |- context[if ?e1 <=! ?e2 then _ else _] ] => 
           destruct (e1 <=! e2) ; try congruence ; try solve [assert False; intuition]; try subst
         | [ |- context[if ?e1 =! ?e2 then _ else _] ] => 
@@ -84,7 +83,18 @@ Module BinaryTreeModel(A : BINARY_TREE_ASSOCIATION).
     intros. destruct (key_cmp k k'); t. 
   Qed.
 
+  Lemma key_lt_imp_ne' : forall k1 k2, k1 < k2 -> k2 <> k1.
+  Proof. intros; pose (key_lt_imp_ne H); auto. Qed.
+  Hint Resolve key_lt_imp_ne key_lt_imp_ne'.
+  
   (* interactions of filter *)
+  Lemma lookup_filter_gte_eq(k:key_t)(l:alist_t) : 
+    lookup k (filter_gte k l) = None.
+  Proof. induction l; t. Qed.
+
+  Lemma lookup_filter_lte_eq(k:key_t)(l:alist_t) : 
+    lookup k (filter_lte k l) = None.
+  Proof. induction l; t. Qed.
 
   Lemma lookup_filter_gte(k1 k2:key_t)(l:alist_t) : 
     k1 < k2 -> lookup k1 (filter_gte k2 l) = lookup k1 l.
@@ -93,12 +103,21 @@ Module BinaryTreeModel(A : BINARY_TREE_ASSOCIATION).
   Lemma lookup_filter_lte(k1 k2:key_t)(l:alist_t) : 
     k2 < k1 -> lookup k1 (filter_lte k2 l) = lookup k1 l.
   Proof. induction l; t. Qed.
-  Hint Rewrite lookup_filter_gte using solve[t] : AssocListModel.
-  Hint Rewrite lookup_filter_lte using solve[t] : AssocListModel.
+  Hint Rewrite lookup_filter_gte_eq lookup_filter_lte_eq : AssocListModel.
+  Hint Rewrite lookup_filter_gte lookup_filter_lte using solve[t] : AssocListModel.
 
   Lemma filter_lookup_none f k l : lookup k l = None -> lookup k (filter f l) = None.
   Proof. induction l; t. Qed.
   Hint Resolve filter_lookup_none.
+
+  Lemma filter_lookup_some_false f k v l : lookup k (filter f l) = Some v -> f k = false.
+  Proof. induction l; t. Qed.
+
+  Lemma filter_lookup_some f k v l : lookup k (filter f l) = Some v -> lookup k l = Some v.
+  Proof. induction l; t; [| destruct (f x); t].
+    case_eq (f k); intro eq1; rewrite eq1 in H0; t.
+    rewrite (filter_lookup_some_false _ _ H0) in eq1. congruence.
+  Qed.
 
   Lemma filter_perm f l l' : Permutation l l' -> Permutation (filter f l) (filter f l').
   Proof. induction 1; t; eauto. Qed.
@@ -139,6 +158,62 @@ Module BinaryTreeModel(A : BINARY_TREE_ASSOCIATION).
   Lemma insert_filter_gte_lt k1 k2 (v:value_t k1) l : k1 < k2 -> (filter_gte k2 (insert v l)) = insert v (filter_gte k2 l).
   Proof. unfold insert; induction l; t. Qed.
   Hint Rewrite insert_filter_gte_lt using solve[t] : AssocListModel.
+
+  (* generally, we will have that lookup k = Some v *)
+  Definition pivot k v l := ((k,,v)::(filter_lte k l) ++ (filter_gte k l)).
+  Implicit Arguments pivot [].
+
+  Lemma pivot_distinct : forall k v l, distinct l -> distinct (pivot k v l).
+  Proof. constructor. t. induction l; t.
+    assert (p:Permutation ((x,, v0) :: (filter_lte k) l ++ (filter_gte k) l)
+      ((filter_lte k) l ++ (x,, v0) :: (filter_gte k) l)).
+      apply Permutation_cons_app; apply Permutation_refl.
+    apply (distinct_perm p). constructor; t.
+  Qed.
+
+  Lemma lookup_app_some1 k v l1 l2 : lookup k l1 = Some v -> lookup k (l1++l2) = Some v.
+  Proof. induction l1; t. Qed.
+
+  Lemma lookup_app_inv k v l1 l2 : lookup k (l1++l2) = Some v -> 
+    lookup k l1 = Some v \/ lookup k l1 = None /\ lookup k l2 = Some v.
+  Proof. induction l1; t. Qed.
+
+  Lemma lookup_filters k k' l : k <> k' -> lookup k l = lookup k ((filter_lte k') l ++ (filter_gte k' l)).
+  Proof. intros. remember (lookup k l) as x. destruct x.
+    remember (lookup k (filter_lte k' l)) as x. destruct x.
+    rewrite (filter_lookup_some _ _ (sym_eq Heqx0)) in Heqx. simpler. 
+    symmetry. eapply lookup_app_some1; eauto.
+    
+
+
+    
+
+      
+
+    destruct (k <=! k'); intuition; try congruence.
+    
+
+         induction l; repeat progress (simpler; simpl in *; intuition).
+         
+
+         induction l; auto. repeat progress (simpler; simpl in *; intuition).
+  Lemma pivot_perm k v l : distinct l -> lookup k l = Some v -> Permutation l (pivot k v l).
+  Proof. intros. apply distinct_look_perm; repeat (progress (simpler; intuition)); unfold pivot.
+         rewrite lookup_app_none1; t.
+         pose (pivot_distinct v l H); firstorder.
+
+
+
+
+
+         
+         
+
+         symmetry; rewrite lookup_app_none1; eapply filter_lookup_none; auto.
+         
+         
+
+
 
 (*
   Lemma insert_filter_lte_lt k1 k2 (v:value_t k1) l : k1 < k2 -> (filter_lte k2 (insert v l)) = (filter_lte k2 l).
@@ -242,8 +317,8 @@ Module BinaryTree(BT : BINARY_TREE_ASSOCIATION). (* : FINITE_MAP with Module A :
     
   Ltac unfolder := idtac; apply rep2node_prem.
   Ltac impsimpler := search_conc ltac:(apply rep2node_conc).
-  Ltac t := unfold rep; unfold_local; repeat progress 
-    (sep ltac:(idtac; search_prem unfolder) AL.simpler; auto; impsimpler; autorewrite with AssocListModel; simpler).
+  Ltac t := unfold rep; unfold_local; repeat progress (
+    repeat progress (sep ltac:(idtac; search_prem unfolder) AL.simpler; auto; impsimpler); simpler; autorewrite with AssocListModel).
 
   (* The new operation: just allocate a ref and initialize it with None *)
   Definition new : T.new.
@@ -261,6 +336,242 @@ Module BinaryTree(BT : BINARY_TREE_ASSOCIATION). (* : FINITE_MAP with Module A :
      Else free (n_left n) (l ~~~ (filter_gte (node_key n) l)) <@> _
        ;; free (n_right n) (l ~~~ (filter_lte (node_key n) l))))
   ; t; t. Qed.
+
+(* debugging tools *)
+Ltac print_goal := idtac; 
+  match goal with
+    [|- ?g] => idtac g
+  end. 
+
+Ltac print_hyps := idtac; 
+  try match goal with
+        [H: ?g |- _] => idtac H ": " g; fail
+end.
+Ltac print_all := idtac ""; idtac "subgoal: "; print_hyps; idtac "========================="; print_goal.
+
+
+
+  Definition remove : T.remove.
+  refine(Fix3 _ _ (fun (remove:T.remove) f k l =>
+     n <- ! f 
+   ; IfNull n
+     Then {{ Return tt}}
+     Else let l_left := (l ~~~ (filter_gte (node_key n) l)) in
+          let l_right := (l ~~~ (filter_lte (node_key n) l)) in
+            Compare BT.key_cmp k (node_key n)
+            WhenLt {{remove (node_left n) k l_left
+              <@> (f --> Some n * (l_right ~~ rep' (node_right n) l_right) * 
+                (l ~~ [AL.lookup (node_key n) l = Some (node_value n)]))}}
+            WhenEq (*Assert (
+              (Exists ln :@ option node_t, (node_left n) --> ln * (l_left ~~ node_rep ln l_left) *
+                f --> Some n * 
+              (l_right ~~ rep' (node_right n) l_right) * 
+              (l ~~ [lookup (node_key n) l = Some (node_value n)])))
+                ;; *) ln <- SepRead (node_left n) 
+                (fun ln => (l_left ~~ node_rep ln l_left) *
+                  f --> Some n * (l_right ~~ rep' (node_right n) l_right) * 
+                  (l ~~ [lookup (node_key n) l = Some (node_value n)]))
+                 ; rn <- SepRead (node_right n)
+                 (fun rn => ((node_left n) --> ln * (l_left ~~ node_rep ln l_left)) *
+                   f --> Some n * (l_right ~~ node_rep rn  l_right) * 
+                  (l ~~ [lookup (node_key n) l = Some (node_value n)]))
+                 ; IfNull ln
+                   Then Free (node_right n)
+                     ;; Free (node_left n)
+                     ;; {{f ::= rn}}
+                    Else {{ remove f k l }}
+            WhenGt {{remove (node_right n) k l_right
+              <@> (f --> Some n * (l_left ~~ rep' (node_left n) l_left) * (l ~~ [AL.lookup (node_key n) l = Some (node_value n)]))}})).
+
+t. t. t. t. t. t. t. t. t. t. t. t. t. t. t. t.
+
+sep fail auto.
+
+
+t. t. t. t. t.
+
+sep fail auto.
+t. 
+t.
+
+
+Ltac equate e1 e2 := not_eq e1 e2; idtac "noteq"; let H := fresh in assert (H : e1 = e2); [idtac "done1"; print_all; 
+  (reflexivity||
+    idtac; match goal with | [|- ?a = ?b] => reflexivity end ||
+idtac "reflexivity failed"; fail) | idtac "done2"; clear H]; idtac "done3". 
+
+
+Ltac equater := idtac "equater called"; force_unify;
+  match goal with
+    | [ |- ?p ==> ?q ] => equate p q || let q := deExist q in equate p q
+    | [ |- (_ _ * __)%hprop ==> _] => idtac "eqs"; apply himp_comm_prem; apply himp_empty_prem; idtac "eqe"; print_all; equater
+    | [ |- _ ==> (_ _ * __)%hprop ] => apply himp_comm_conc; apply himp_empty_conc; equater
+    | [ |- ?p ==> (?q * __)%hprop ] => equate p q || let q := deExist q in equate p q
+    | [ |- (?p * __)%hprop ==> ?q ] => equate p q || let q := deExist q in equate p q
+    | [ |- ?U ?X ==> ?p ] =>
+      let H := fresh in
+        (pose (H := p); pattern X in H;
+          assert (H' : H = H); [
+            cbv delta [H]; match goal with
+                             | [ |- ?F _ = _ ] => equate U F
+                           end; reflexivity
+            | idtac
+          ]; clear H H'); simpl; try apply himp_refl
+    | [ |- ?p ==> ?U ?X ] => idtac "in fun equater ";
+      let H := fresh in
+        (pose (H := p); print_all; pattern X in H; 
+          assert (H' : H = H); [ idtac "after pattern"; print_all;
+            cbv delta [H]; match goal with
+                             | [ |- ?F _ = _ ] => idtac "equater match"; idtac "U: " U "F: " F; equate U F
+                           end; reflexivity
+            | simpl; idtac "equator success"; try apply himp_refl
+          ]; clear H H')
+  end.
+
+Ltac sep stac tac :=
+  let s := repeat progress (simpler; tac; try search_prem premer) in
+    let concer := apply himp_empty_conc
+      || apply himp_ex_conc_trivial
+        || (apply himp_ex_conc; econstructor)
+          || (eapply himp_unpack_conc; [eassumption || reflexivity |])
+            || (apply himp_inj_conc; [s; fail | idtac]) in
+              (intros; equater || specFinder stac; tac;
+                repeat match goal with
+                         | [ x : inhabited _ |- _ ] => dependent inversion x; clear x
+                       end;
+                intros; s;
+                  repeat ((
+                    search_prem ltac:(idtac;
+                      search_conc ltac:(
+                        (apply himp_frame; trivial; force_unify; idtac "himp_frame applied, trying to equate"; print_all; equater; idtac "equated!"; force_unify; print_goal) || (apply himp_frame_cell; trivial))) || search_conc concer); 
+                  s);
+                  try finisher).
+
+  Lemma rep2node_conc'(x:fmap_t)(l:AL.alist_t) P Q: 
+  P ==> rep' x l * Q -> P ==> (Exists n :@ option node_t, x --> n * node_rep n l * Q).
+  Proof. intros. eapply himp_trans. eexact H. t. Qed.
+
+  Lemma rep2node_conc''(x:fmap_t)(l:AL.alist_t) P: 
+  P ==> rep' x l -> P ==> (Exists n :@ option node_t, x --> n * node_rep n l).
+  Proof. intros. eapply himp_trans. eexact H. t. Qed.
+
+sep fail print_goal.
+
+assert (exists HH, (node_rep v x2 * (f --> Some n0 * rep' (node_right n0) x3) ==> HH v * __)). econstructor.
+sep fail auto.
+
+assert (exists FF, exists GG, exists HH, exists II, 
+  (node_left n0 --> v * ((f --> Some n0 * node_rep v HH) *
+ rep' (node_right n0) GG)) ==>
+ (Exists v :@ option FF, node_left n0 --> v * II v)).
+do 4 econstructor. 
+apply himp_empty_conc'. apply himp_ex_conc. econstructor.
+apply himp_assoc_conc1.
+apply himp_frame; equater.
+
+
+
+
+
+
+equater.
+
+
+Ltac equater2 := force_unify;
+  match goal with
+    | [ |- ?p ==> ?q ] => equate p q || let q := deExist q in equate p q
+    | [ |- ?p ==> (?q * __)%hprop ] => equate p q || let q := deExist q in equate p q
+    | [ |- (?p * __)%hprop ==> ?q ] => equate p q || let q := deExist q in equate p q
+    | [ |- ?U ?X ==> ?p ] =>
+      let H := fresh in
+        (pose (H := p); pattern X in H;
+          assert (H' : H = H); [
+            cbv delta [H]; match goal with
+                             | [ |- ?F _ = _ ] => equate U F
+                           end; reflexivity
+            | idtac
+          ]; clear H H')
+    | [ |- ?p ==> ?U ?X ] =>
+      let H := fresh in
+        (pose (H := p); pattern X in H;
+          assert (H' : H = H); [
+            cbv delta [H]; match goal with
+                             | [ |- ?F _ = _ ] => equate U F
+                           end; reflexivity
+            | simpl; try apply himp_refl
+          ]; clear H H')
+    | [ |- (_ _ * __)%hprop ==> _] => apply himp_comm_prem; apply himp_empty_prem; equater2
+    | [ |- _ ==> (_ * __)%hprop ] => idtac "equ"; apply himp_comm_conc; apply himp_empty_conc; idtac "equ2"; print_goal; equater2
+  end.
+
+
+
+
+
+Ltac equater3 := 
+  match goal with
+    | [ |- ?p ==> ?U ?X ] => idtac "eqpat"; idtac "p: " p " U: " U  " X: " X;
+      let H := fresh in
+        (pose (H := p); pattern X in H;
+          assert (H' : H = H); [idtac "solv_eq: "; idtac H; print_all;
+            cbv delta [H]; idtac "delta"; print_all; match goal with
+                             | [ |- ?F _ = _ ] => idtac "inrefl"; equate U F; idtac "end_refl"
+                           end; reflexivity
+            | idtac "after refl"; print_all; idtac; simpl; try apply himp_refl
+          ]; clear H H')
+  end.
+
+
+equater3.
+
+
+match goal with
+  | [ |- ?p ==> ?U ?X ] => idtac "eqpat"; idtac "p: " p " U: " U  " X: " X;
+    let H := fresh in
+      (pose (H := p); pattern X in H;
+        assert (H' : H = H); [idtac "solv_eq: "; idtac H; print_all;
+          cbv delta [H]; idtac "delta"; print_all; match goal with
+                                                     | [ |- ?F _ = _ ] => idtac "inrefl"; equate U F; idtac "end_refl"
+                                                   end; reflexivity
+            | idtac "after refl"; print_all; idtac; 
+        ]; clear H H')
+end.
+
+
+
+
+; ; force_unify; print_goal.
+
+match goal with 
+  [|- ?p * ?q1 ==> ?p * ?q2] => apply (@himp_frame p q1 q2)
+end.
+
+; print_goal; simpl; print_goal.
+
+
+
+pose (H8:=Some n0).
+pattern n0 in H8.
+          assert (H' : H = H); [
+            cbv delta [H]; match goal with
+                             | [ |- ?F _ = _ ] => equate U F
+                           end; reflexivity
+            | idtac
+          ]; clear H H')
+(node_rep v ?7184 * (f --> Some n0 * rep' (node_right n0) ?7185) ==>
+ ?3292 ?7378 * __)
+
+assert (exists HH, exists GG, (
+  (hprop_imp
+   (hprop_sep (node_rep v x)
+      (hprop_sep (@hprop_cell f (option node_t) (@Some node_t n0))
+         (rep' (node_right n0) x))) (hprop_sep (GG HH) hprop_empty)))).
+
+node_rep v HH * (f --> Some n0 * rep' (node_right n0) GG) ==>
+ FF II * __)).
+
+
+subst n; simpl.
 
   Definition lookup  : T.lookup.
   refine (Fix3 _ _ (fun (lookup:T.lookup) f k l => 
@@ -292,6 +603,6 @@ Module BinaryTree(BT : BINARY_TREE_ASSOCIATION). (* : FINITE_MAP with Module A :
             WhenEq {{ f ::= Some (Node v (node_left n) (node_right n)) }}
             WhenGt {{insert (node_right n) k v l_right
               <@> (f --> Some n * (l_left ~~ rep' (node_left n) l_left) * (l ~~ [AL.lookup (node_key n) l = Some (node_value n)]))}}))
- ; t. Qed.
+ ; t; intuition; t. Qed.
 
 End BinaryTree.
